wah

lib/STLC/Has.v
@@ -20,8 +20,7 @@ Inductive term : list type -> type -> Set :=
   Γ ⊢ τ'
 where "Γ '⊢' τ" := (term Γ τ) : type_scope.
 
-Derive Signature for term.
-Equations Derive NoConfusion NoConfusionHom Subterm for term.
+Equations Derive Signature NoConfusion NoConfusionHom Subterm for term.
 
 Declare Scope term_scope.
 Delimit Scope term_scope with term.
@@ -60,3 +59,62 @@ Equations
   subs f (Id _ _ h)   := f _ h;
   subs f (λ ρ ⇒ t')%term := (`λ subs (fun τ => Exts f ρ (σ:=τ)) t')%term;
   subs f (t₁ ⋅ t₂)%term  := (subs f t₁ ⋅ subs f t₂)%term.
+
+Equations sub_helper : forall {Γ τ}, Γ ⊢ τ -> forall τ', Has τ' (τ :: Γ) -> Γ ⊢ τ' :=
+  sub_helper t _ HasO := t;
+  sub_helper _ _ (HasS hs) := Id _ _ hs.
+
+Definition sub {Γ τ τ'} (body : τ :: Γ ⊢ τ') (arg : Γ ⊢ τ) : Γ ⊢ τ' :=
+    subs (sub_helper arg) body.
+
+Notation "x '[[' y ']]'"
+  := (sub x y) (at level 12, no associativity) : term_scope.
+
+Reserved Notation "x '-->' y" (at level 80, no associativity).
+
+Inductive bred {Γ} : forall {τ}, Γ ⊢ τ -> Γ ⊢ τ -> Prop :=
+| bred_bred τ τ' (t₁ : τ :: Γ ⊢ τ') t₂ :
+    ((`λ t₁) ⋅ t₂)%term --> (t₁ [[ t₂ ]])%term
+| bred_abs τ τ' (t t' : τ :: Γ ⊢ τ') :
+    t -->  t' ->
+    (`λ t)%term --> (`λ t')%term
+| bred_app_l τ τ' (t₁ t₁' : Γ ⊢ τ → τ') t₂ :
+    t₁ -->  t₁' ->
+    (t₁ ⋅ t₂)%term -->  (t₁' ⋅ t₂)%term
+| bred_app_r τ τ' (t₁ : Γ ⊢ τ → τ') t₂ t₂' :
+    t₂ -->  t₂' ->
+    (t₁ ⋅ t₂)%term -->  (t₁ ⋅ t₂')%term
+where "x '-->' y" := (bred x y) : type_scope.
+
+Print Assumptions bred.
+
+Local Hint Constructors bred : core.
+
+Variant value {Γ : list type} : forall {τ : type}, Γ ⊢ τ -> Prop :=
+  Abs_value (τ τ' : type) (t : τ :: Γ ⊢ τ') : value (`λ t)%term.
+Derive Signature for value.
+
+Print Assumptions value.
+
+Lemma canonical_forms_abs : forall {τ τ' : type} (t : [] ⊢ (τ → τ')%ty),
+    value t -> exists body : [τ] ⊢ τ', t = (`λ body)%term.
+Proof.
+  intros τ τ' t v.
+  depelim v; eauto.
+Qed.
+
+Print Assumptions canonical_forms_abs.
+
+Local Hint Constructors bred : core.
+Local Hint Constructors value : core.
+
+Lemma Progress : forall {τ} (t : [] ⊢ τ), value t \/ exists t', t --> t'.
+Proof.
+  intros τ t; depind t; eauto.
+  - inv h.
+  - clear IHt2.
+    destruct IHt1 as [v1 | (t1' & ih1)]; eauto.
+    apply canonical_forms_abs in v1 as [t1' ?]; subst; eauto.
+Qed.
+
+Print Assumptions Progress.
